plugins/lean_meta/lean_meta_smt_model.lean
@@ -1,0 +1,223 @@
+import Cpc.SmtEval
+
+set_option linter.unusedVariables false
+
+namespace SmtModel
+
+/- SMT literal evaluation defined -/
+
+abbrev smt_lit_Bool := SmtEval.smt_lit_Bool
+abbrev smt_lit_Int := SmtEval.smt_lit_Int
+abbrev smt_lit_Rat := SmtEval.smt_lit_Rat
+abbrev smt_lit_String := SmtEval.smt_lit_String
+abbrev smt_lit_RegLan := SmtEval.smt_lit_String --FIXME
+
+def smt_lit_ite {T : Type} (c : smt_lit_Bool) (t e : T) : T :=
+  if c then t else e
+abbrev smt_lit_not := SmtEval.smt_lit_not
+abbrev smt_lit_and := SmtEval.smt_lit_and
+abbrev smt_lit_iff := SmtEval.smt_lit_iff
+abbrev smt_lit_or := SmtEval.smt_lit_or
+abbrev smt_lit_xor := SmtEval.smt_lit_xor
+abbrev smt_lit_zplus := SmtEval.smt_lit_zplus
+abbrev smt_lit_zmult := SmtEval.smt_lit_zmult
+abbrev smt_lit_zneg := SmtEval.smt_lit_zneg
+abbrev smt_lit_zeq := SmtEval.smt_lit_zeq
+abbrev smt_lit_zleq := SmtEval.smt_lit_zleq
+abbrev smt_lit_zlt := SmtEval.smt_lit_zlt
+abbrev smt_lit_div := SmtEval.smt_lit_div
+abbrev smt_lit_mod := SmtEval.smt_lit_mod
+abbrev smt_lit_int_pow2 := SmtEval.smt_lit_int_pow2
+abbrev smt_lit_piand := SmtEval.smt_lit_piand
+abbrev smt_lit_mk_rational := SmtEval.smt_lit_mk_rational
+abbrev smt_lit_qplus := SmtEval.smt_lit_qplus
+abbrev smt_lit_qmult := SmtEval.smt_lit_qmult
+abbrev smt_lit_qneg := SmtEval.smt_lit_qneg
+abbrev smt_lit_qeq := SmtEval.smt_lit_qeq
+abbrev smt_lit_qleq := SmtEval.smt_lit_qleq
+abbrev smt_lit_qlt := SmtEval.smt_lit_qlt
+abbrev smt_lit_qdiv := SmtEval.smt_lit_qdiv
+abbrev smt_lit_to_int := SmtEval.smt_lit_to_int
+abbrev smt_lit_to_real := SmtEval.smt_lit_to_real
+abbrev smt_lit_str_len := SmtEval.smt_lit_str_len
+abbrev smt_lit_str_concat := SmtEval.smt_lit_str_concat
+abbrev smt_lit_str_substr := SmtEval.smt_lit_str_substr
+abbrev smt_lit_str_indexof := SmtEval.smt_lit_str_indexof
+abbrev smt_lit_str_to_code := SmtEval.smt_lit_str_to_code
+abbrev smt_lit_str_from_code := SmtEval.smt_lit_str_from_code
+
+abbrev __smtx_pow2 := SmtEval.__smtx_pow2
+abbrev __smtx_bit := SmtEval.__smtx_bit
+abbrev __smtx_msb := SmtEval.__smtx_msb
+abbrev __smtx_binary_or := SmtEval.__smtx_binary_or
+abbrev __smtx_binary_xor := SmtEval.__smtx_binary_xor
+abbrev __smtx_binary_not := SmtEval.__smtx_binary_not
+abbrev __smtx_binary_max := SmtEval.__smtx_binary_max
+abbrev __smtx_binary_uts := SmtEval.__smtx_binary_uts
+abbrev __smtx_binary_concat := SmtEval.__smtx_binary_concat
+abbrev __smtx_binary_extract := SmtEval.__smtx_binary_extract
+
+-- SMT Beyond Eunoia
+
+def smt_lit_streq : smt_lit_String -> smt_lit_String -> smt_lit_Bool
+  | x, y => decide (x = y)
+
+def smt_lit_int_log2 : smt_lit_Int -> smt_lit_Int
+  | _ => 0 -- FIXME
+
+def smt_lit_str_lt : smt_lit_String -> smt_lit_String -> smt_lit_Bool
+  | _, _ => false -- FIXME
+def smt_lit_str_from_int : smt_lit_Int -> smt_lit_String
+  | _ => "" -- FIXME
+def smt_lit_str_to_int : smt_lit_String -> smt_lit_Int
+  | _ => 0 -- FIXME
+def smt_lit_str_to_upper : smt_lit_String -> smt_lit_String
+  | _ => "" -- FIXME
+def smt_lit_str_to_lower : smt_lit_String -> smt_lit_String
+  | _ => "" -- FIXME
+def smt_lit_str_update : smt_lit_String -> smt_lit_Int -> smt_lit_String -> smt_lit_String
+  | _, _, _ => "" -- FIXME
+def smt_lit_str_rev : smt_lit_String -> smt_lit_String
+  | _ => "" -- FIXME
+def smt_lit_str_replace : smt_lit_String -> smt_lit_String -> smt_lit_String -> smt_lit_String
+  | _, _, _ => "" -- FIXME
+def smt_lit_str_replace_all : smt_lit_String -> smt_lit_String -> smt_lit_String -> smt_lit_String
+  | _, _, _ => "" -- FIXME
+def smt_lit_str_contains : smt_lit_String -> smt_lit_String -> smt_lit_Bool
+  | _, _ => false -- FIXME
+def smt_lit_str_to_re : smt_lit_String -> smt_lit_RegLan
+  | _ => "" -- FIXME
+def smt_lit_re_mult : smt_lit_RegLan -> smt_lit_RegLan
+  | _ => "" -- FIXME
+def smt_lit_re_plus : smt_lit_RegLan -> smt_lit_RegLan
+  | _ => "" -- FIXME
+def smt_lit_re_comp : smt_lit_RegLan -> smt_lit_RegLan
+  | _ => "" -- FIXME
+def smt_lit_re_concat : smt_lit_RegLan -> smt_lit_RegLan -> smt_lit_RegLan
+  | _, _ => "" -- FIXME
+def smt_lit_re_inter : smt_lit_RegLan -> smt_lit_RegLan -> smt_lit_RegLan
+  | _, _ => "" -- FIXME
+def smt_lit_re_diff : smt_lit_RegLan -> smt_lit_RegLan -> smt_lit_RegLan
+  | _, _ => "" -- FIXME
+def smt_lit_re_union : smt_lit_RegLan -> smt_lit_RegLan -> smt_lit_RegLan
+  | _, _ => "" -- FIXME
+def smt_lit_re_range : smt_lit_String -> smt_lit_String -> smt_lit_RegLan
+  | _, _ => "" -- FIXME
+def smt_lit_str_in_re : smt_lit_String -> smt_lit_RegLan -> smt_lit_Bool
+  | _, _ => false -- FIXME
+def smt_lit_str_indexof_re : smt_lit_String -> smt_lit_RegLan -> smt_lit_Int -> smt_lit_Int
+  | _, _, _ => 0 -- FIXME
+def smt_lit_str_replace_re : smt_lit_String -> smt_lit_RegLan -> smt_lit_String -> smt_lit_String
+  | _, _, _ => "" -- FIXME
+def smt_lit_str_replace_re_all : smt_lit_String -> smt_lit_RegLan -> smt_lit_String -> smt_lit_String
+  | _, _, _ => "" -- FIXME
+def smt_lit_re_allchar : smt_lit_RegLan := "" --FIXME
+def smt_lit_re_none : smt_lit_RegLan := "" --FIXME
+def smt_lit_re_all : smt_lit_RegLan := "" --FIXME
+
+-- Partial semantics
+
+def smt_lit_qdiv_by_zero : smt_lit_Rat -> smt_lit_Rat
+  | x => x -- FIXME
+def smt_lit_div_by_zero : smt_lit_Int -> smt_lit_Int
+  | x => x -- FIXME
+def smt_lit_mod_by_zero : smt_lit_Int -> smt_lit_Int
+  | x => x -- FIXME
+
+
+mutual
+
+/- 
+SMT-LIB types.
+-/
+inductive SmtType : Type where
+$LEAN_SMT_TYPE_DEF$
+deriving Repr, DecidableEq, Inhabited
+
+/- 
+SMT-LIB terms.
+-/
+inductive SmtTerm : Type where
+$LEAN_SMT_TERM_DEF$
+deriving Repr, DecidableEq, Inhabited
+
+/- 
+SMT-LIB values.
+-/
+inductive SmtValue : Type where
+$LEAN_SMT_VALUE_DEF$
+deriving Repr, DecidableEq, Inhabited
+
+/-
+SMT-LIB map values.
+-/
+inductive SmtMap : Type where
+  | cons : SmtValue -> SmtValue -> SmtMap -> SmtMap
+  | default : SmtType -> SmtValue -> SmtMap
+deriving Repr, DecidableEq, Inhabited
+
+/- 
+SMT-LIB sequence values.
+-/
+inductive SmtSeq : Type where
+  | cons : SmtValue -> SmtSeq -> SmtSeq
+  | empty : SmtType -> SmtSeq
+deriving Repr, DecidableEq, Inhabited
+
+/-
+SMT-LIB datatypes.
+-/
+inductive SmtDatatype : Type where
+  | null : SmtDatatype
+  | sum : SmtDatatypeCons -> SmtDatatype -> SmtDatatype
+deriving Repr, DecidableEq, Inhabited
+
+/-
+SMT-LIB datatype constructors.
+-/
+inductive SmtDatatypeCons : Type where
+  | unit : SmtDatatypeCons
+  | cons : SmtType -> SmtDatatypeCons -> SmtDatatypeCons
+deriving Repr, DecidableEq, Inhabited
+
+end
+
+/- Type equality -/
+def smt_lit_Teq : SmtType -> SmtType -> smt_lit_Bool
+  | x, y => decide (x = y)
+/- Value equality -/
+def smt_lit_veq : SmtValue -> SmtValue -> smt_lit_Bool
+  | x, y => decide (x = y)
+/- Used for ordering values -/
+def __smtx_value_hash : SmtValue -> smt_lit_Int
+  | _ => 0 -- FIXME
+  
+/- exists -/
+def smt_lit_tforall : smt_lit_String -> SmtType -> SmtTerm -> SmtValue
+  | _, _, _ => (SmtValue.Boolean true) -- FIXME
+/- forall -/
+def smt_lit_texists : smt_lit_String -> SmtType -> SmtTerm -> SmtValue
+  | _, _, _ => (SmtValue.Boolean true) -- FIXME
+/- choice -/
+def smt_lit_tchoice : smt_lit_String -> SmtType -> SmtTerm -> SmtValue
+  | _, _, _ => (SmtValue.Boolean true) -- FIXME
+
+/- Definition of SMT-LIB model semantics -/
+
+mutual
+
+$LEAN_SMT_EVAL_DEFS$
+
+end
+
+inductive smt_interprets : SmtTerm -> Bool -> Prop
+  | intro_true  (t : SmtTerm) :
+      (__smtx_model_eval t) = (SmtValue.Boolean true) ->
+      smt_interprets t true
+  | intro_false (t : SmtTerm) :
+      (__smtx_model_eval t) = (SmtValue.Boolean false)->
+      smt_interprets t false
+
+/- ---------------------------------------------- -/
+
+end SmtModel
