plugins/lean_meta/lean_meta_spec.lean
@@ -1,0 +1,75 @@
+import Cpc.SmtModel
+import Cpc.Logos
+
+set_option linter.unusedVariables false
+
+namespace EoCorrect
+
+abbrev Term := Eo.Term
+abbrev CCmdList := Eo.CCmdList
+abbrev SmtType := SmtModel.SmtType
+abbrev SmtTerm := SmtModel.SmtTerm
+
+/- Definitions for theorems -/
+
+/- Definition of refutation -/
+
+inductive eo_is_refutation : Term -> CCmdList -> Prop
+$LEAN_EO_IS_REFUTATION_DEF$
+
+/-
+A definition of terms in the object language.
+This is to be defined externally.
+-/
+abbrev Object_Term := SmtTerm
+
+/-
+A predicate defining a relation on terms in the object language and Booleans
+such that (s,b) is true if s evaluates to b.
+This is to be defined externally.
+-/
+abbrev obj_interprets := smt_interprets
+
+
+/-
+Definitions for eo_is_obj
+-/
+mutual
+
+$LEAN_EO_IS_OBJ_DEFS$
+
+end 
+
+/-
+An inductive predicate defining the correspondence between Eunoia terms
+and terms in the object language.
+(t,s) is true if the Eunoia term represents a term s in the object language.
+This is to be custom defined in the Eunoia-to-Lean compiler based on the
+target definition of Object_Term.
+-/
+inductive eo_is_obj : Term -> Object_Term -> Prop
+$LEAN_EO_IS_OBJ$
+
+/-
+A predicate defining when a Eunoia term corresponds to an object term that
+evaluates to true or false.
+(t,b) is true if t is a Eunoia term corresponding to an object term that
+evaluates to b.
+-/
+def eo_interprets (t : Term) (b : Bool) : Prop :=
+  exists (s : Object_Term), (eo_is_obj t s) /\ (obj_interprets s b)
+
+/- The theorem statements -/
+
+$LEAN_THMS$
+
+/- correctness theorem for the checker -/
+theorem correct___eo_is_refutation (F : Term) (pf : CCmdList) :
+  (eo_is_refutation F pf) ->
+  (Not (eo_interprets F true)) :=
+by
+  sorry
+
+/- ---------------------------------------------- -/
+
+end EoCorrect
